LeanSAT/Reflect/BoolExpr/Tseitin.lean
@@ -13,6 +13,14 @@ import Std.Tactic.LibrarySearch
 @[simp] theorem true_beq_false : (true == false) = false := rfl
 @[simp] theorem true_beq_true : (true == true) = true := rfl
 
+@[simp] theorem false_beq : (false == x) = !x := by cases x <;> simp
+@[simp] theorem beq_false : (x == false) = !x := by cases x <;> simp
+@[simp] theorem true_beq : (true == x) = x := by cases x <;> simp
+@[simp] theorem beq_true : (x == true) = x := by cases x <;> simp
+
+theorem eq_true_or_eq_false {x : Bool} : x = true ∨ x = false := by cases x <;> simp
+theorem eq_false_or_eq_true {x : Bool} : x = false ∨ x = true := by cases x <;> simp
+
 namespace Gate
 
 def toCNF (i₁ i₂ o : α) : Gate → CNF α
@@ -29,15 +37,18 @@ def toCNF (i₁ i₂ o : α) : Gate → CNF α
   | .imp =>
     [[(o, true), (i₁, true), (i₂, false)], [(o, false), (i₁, false)], [(o, false), (i₂, true)]]
 
-theorem toCNF_sat : (toCNF i₁ i₂ o g).sat f ↔ f o = g.eval (f i₁) (f i₂) := by
+@[simp] theorem toCNF_eval {i₁ i₂ o : α} : (toCNF i₁ i₂ o g).eval f = (f o == g.eval (f i₁) (f i₂)) := by
   match g with
   | .and
   | .or
   | .xor
   | .beq
   | .imp =>
-    simp [toCNF, eval, CNF.sat, CNF.eval, CNF.Clause.eval]
+    simp [toCNF, eval, CNF.eval, CNF.Clause.eval]
     cases f o <;> cases f i₁ <;> cases f i₂ <;> simp
+
+theorem toCNF_sat : (toCNF i₁ i₂ o g).sat f ↔ f o = g.eval (f i₁) (f i₂) := by
+  simp [CNF.sat]
 
 end Gate
 
@@ -45,15 +56,20 @@ namespace CNF
 
 def eq (x y : α) : CNF α := [[(x, true), (y, false)], [(x, false), (y, true)]]
 
-theorem eq_sat : (eq x y).sat f ↔ f x = f y := by
-  simp [eq, eval, CNF.sat, CNF.eval, CNF.Clause.eval]
+@[simp] theorem eq_eval : (eq x y).eval f = (f x == f y) := by
+  simp [eq, CNF.eval, CNF.Clause.eval]
   cases f x <;> cases f y <;> simp
+
+theorem eq_sat : (eq x y).sat f ↔ f x = f y := by simp [CNF.sat]
 
 def ne (x y : α) : CNF α := [[(x, true), (y, true)], [(x, false), (y, false)]]
 
-theorem ne_sat : (ne x y).sat f ↔ f x = !f y := by
-  simp [ne, eval, CNF.sat, CNF.eval, CNF.Clause.eval]
+@[simp] theorem ne_eval : (ne x y).eval f = (f x == !f y) := by
+  simp [ne, CNF.eval, CNF.Clause.eval]
   cases f x <;> cases f y <;> simp
+
+theorem ne_sat : (ne x y).sat f ↔ f x = !f y := by simp [CNF.sat]
+
 end CNF
 
 namespace BoolExpr
@@ -83,37 +99,212 @@ We produce a CNF with literals labelled by `α ⊕ Nat`.
   a gate (0-ary, 1-ary, or 2-ary) in the `BoolExpr`.
 -/
 def toCNF' (x : BoolExpr α) : CNF (α ⊕ Nat) :=
-  let (_, c, p) := run 0 x
-  [(p, false)] :: c
+  let (c, p) := run 0 x
+  [(.inr p, false)] :: c
 where
   /--
   We take as additional argument `k : Nat` which is the "next available circuit node label"
   and return an `α ⊕ Nat`, the label of the "output node".
   -/
-  run (k : Nat) : BoolExpr α → Nat × CNF (α ⊕ Nat) × (α ⊕ Nat)
-  | .literal a => (k + 1, CNF.eq (.inl a) (.inr k), .inr k)
-  | .const b => (k + 1, [[(.inr k, !b)]], .inr k)
+  run (k : Nat) : BoolExpr α → CNF (α ⊕ Nat) × Nat
+  | .literal a => (CNF.eq (.inl a) (.inr k), k)
+  | .const b => ([[(.inr k, !b)]], k)
   | .not x => match run k x with
-    | (k', c, p) => (k' + 1, CNF.ne (.inr k') p ++ c, .inr k')
+    | (c, nx) => (CNF.ne (.inr (nx + 1)) (.inr nx) ++ c, nx + 1)
   | .gate g x y => match run k x with
-    | (kx, cx, px) => match run kx y with
-      | (ky, cy, py) =>
-        (ky + 1, g.toCNF px py (.inr ky) ++ cx ++ cy, .inr ky)
+    | (cx, nx) => match run (nx + 1) y with
+      | (cy, ny) =>
+        (g.toCNF (.inr nx) (.inr ny) (.inr (ny + 1)) ++ cx ++ cy, ny + 1)
 
-theorem toCNF'_run_eval (k : Nat) (x : BoolExpr α) :
-    let (_, c, p) := toCNF'.run k x
-    c.eval f = (x.eval (fun a => f (.inl a)) == f p) :=
-  sorry
+@[simp] theorem toCNF'_run_snd (x : BoolExpr α) : (toCNF'.run k x).2 = k + x.size - 1 := by
+  match x with
+  | .literal _
+  | .const _
+  | .not x
+  | .gate _ x y =>
+    have := x.size_pos
+    simp [toCNF'.run, size, toCNF'_run_snd] <;> omega
 
-theorem toCNF'_eval {x : BoolExpr α} : (toCNF' x).eval f = x.eval (fun a => f (.inl a)) :=
-  sorry
+theorem toCNF'_run_eval (k : Nat) (x : BoolExpr α) (f : α ⊕ Nat → Bool) :
+    let (c, p) := toCNF'.run k x
+    !(c.eval f) || (x.eval (fun a => f (.inl a)) == f (.inr p)) := by
+  match x with
+  | .literal a => simp [toCNF'.run]
+  | .const b => simp [toCNF'.run] <;> cases b <;> cases f (Sum.inr k) <;> simp
+  | .not x =>
+    dsimp only [toCNF'.run]
+    have := toCNF'_run_eval k x f
+    revert this
+    simp
+    generalize f (.inr _) = x1
+    generalize f (.inr _) = x2
+    generalize eval (fun a => f (Sum.inl a)) x = x3
+    generalize CNF.eval f (toCNF'.run k x).fst = x4
+    cases x1 <;> cases x2 <;> simp
+  | .gate g x y =>
+    dsimp only [toCNF'.run]
+    have := toCNF'_run_eval k x f
+    revert this
+    have := toCNF'_run_eval ((toCNF'.run k x).2 + 1) y f
+    revert this
+    simp
+    generalize f (.inr _) = x1
+    generalize f (.inr _) = x2
+    generalize f (.inr _) = x3
+    generalize eval (fun a => f (Sum.inl a)) x = x4
+    generalize eval (fun a => f (Sum.inl a)) y = x5
+    generalize CNF.eval f _ = x6
+    generalize CNF.eval f _ = x7
+    cases x1 <;> cases x2 <;> cases x3 <;> cases x4 <;> cases x5 <;> cases x6 <;> cases x7
+      <;> simp [eq_true_or_eq_false, eq_false_or_eq_true]
+
+theorem toCNF'_eval (x : BoolExpr α) (f : α ⊕ Nat → Bool) :
+    !(toCNF' x).eval f || x.eval (fun a => f (.inl a)) := by
+  dsimp [toCNF']
+  have := toCNF'_run_eval 0 x f
+  revert this
+  simp
+  generalize f (.inr _) = x1
+  generalize eval (fun a => f (Sum.inl a)) x = x2
+  cases x1 <;> cases x2 <;> simp
 
 -- the output of the `k`-th gate
-def traceEval (x : BoolExpr α) (f : α → Bool) (k : Nat) : Bool := sorry
+def traceEval (x : BoolExpr α) (f : α → Bool) (l : Nat) : Bool :=
+  (run 0 x).1
+where
+  run (k : Nat) : BoolExpr α → Bool × Bool × Nat
+  | .literal a => (f a, k = l, k)
+  | .const b => (b, k = l, k)
+  | .not x => match run k x with
+    | (r, d, k') => (bif d then r else !r, d || (k' + 1 = l), k' + 1)
+  | .gate g x y => match run k x with
+    | (rx, dx, kx) => match run (kx + 1) y with
+      | (ry, dy, ky) =>
+        (bif dx then rx else bif dy then ry else g.eval rx ry, dx || dy || (ky + 1 = l), ky + 1)
 
-theorem toCNF'_eval_elim_traceEval {x : BoolExpr α} (f : α → Bool) :
-    (toCNF' x).eval (Sum.elim f (x.traceEval f)) = x.eval f :=
-  sorry
+theorem traceEval_run_snd_snd : (traceEval.run f l k x).2.2 = k + x.size - 1 := by
+  match x with
+  | .literal _ => simp [size, traceEval.run]
+  | .const _ => simp [size, traceEval.run]
+  | .not x =>
+    have := x.size_pos
+    simp only [size, traceEval.run] at *
+    rw [traceEval_run_snd_snd] <;> omega
+  | .gate g x y =>
+    have := x.size_pos
+    have := y.size_pos
+    simp only [size, traceEval.run] at *
+    rw [traceEval_run_snd_snd, traceEval_run_snd_snd]
+    all_goals omega
+
+theorem traceEval_run_snd_fst_of_le (w : k + x.size ≤ l) : (traceEval.run f l k x).2.1 = false := by
+  match x with
+  | .literal a => simp [size, traceEval.run] at * <;> omega
+  | .const b => simp [size, traceEval.run] at * <;> omega
+  | .not x =>
+    have := x.size_pos
+    simp only [size, traceEval.run] at *
+    rw [traceEval_run_snd_fst_of_le]
+    simp only [Bool.false_or, decide_eq_false_iff_not, ne_eq]
+    rw [traceEval_run_snd_snd]
+    all_goals omega
+  | .gate g x y =>
+    have := x.size_pos
+    have := y.size_pos
+    simp only [size, traceEval.run] at *
+    rw [traceEval_run_snd_snd, traceEval_run_snd_snd, traceEval_run_snd_fst_of_le,
+      traceEval_run_snd_fst_of_le]
+    simp only [Bool.or_self, Bool.false_or, decide_eq_false_iff_not, ne_eq]
+    all_goals omega
+
+theorem traceEval_run_snd_fst (w₁ : k ≤ l) (w₂ : l < k + x.size) : (traceEval.run f l k x).2.1 = true := by
+  match x with
+  | .literal a => simp [size, traceEval.run] at * <;> omega
+  | .const b => simp [size, traceEval.run] at * <;> omega
+  | .not x =>
+    have := x.size_pos
+    simp only [size, traceEval.run] at *
+    rw [traceEval_run_snd_snd]
+    by_cases w₃ : l < k + x.size
+    · rw [traceEval_run_snd_fst]
+      simp only [Bool.true_or]
+      all_goals omega
+    · rw [traceEval_run_snd_fst_of_le]
+      simp only [Bool.false_or, decide_eq_true_eq]
+      all_goals omega
+  | .gate g x y =>
+    have := x.size_pos
+    have := y.size_pos
+    simp only [size, traceEval.run] at *
+    rw [traceEval_run_snd_snd, traceEval_run_snd_snd]
+    by_cases w₃ : l < k + x.size
+    · rw [traceEval_run_snd_fst]
+      simp only [Bool.true_or]
+      all_goals omega
+    · rw [traceEval_run_snd_fst_of_le]
+      simp only [Bool.false_or, Bool.or_eq_true, decide_eq_true_eq]
+      by_cases w₄ : l < k + x.size + y.size
+      · rw [traceEval_run_snd_fst]
+        simp only [true_or]
+        all_goals omega
+      · rw [traceEval_run_snd_fst_of_le]
+        simp only [false_or]
+        all_goals omega
+      omega
+
+theorem traceEval_run_fst (w : k + x.size - 1 ≤ l) : (traceEval.run f l k x).1 = x.eval f := by
+  match x with
+  | .literal a => simp [size, traceEval.run]
+  | .const b => simp [size, traceEval.run]
+  | .not x =>
+    have := x.size_pos
+    simp [size, traceEval.run] at *
+    rw [traceEval_run_snd_fst_of_le, traceEval_run_fst]
+    simp only [cond_false]
+    all_goals omega
+  | .gate g x y =>
+    have := x.size_pos
+    have := y.size_pos
+    simp [size, traceEval.run] at *
+    rw [traceEval_run_snd_snd, traceEval_run_snd_fst_of_le, traceEval_run_snd_fst_of_le,
+      traceEval_run_fst, traceEval_run_fst]
+    simp only [cond_false]
+    all_goals omega
+
+theorem toCNF'_run_fst_eval_elim_traceEval (x : BoolExpr α) (f : α → Bool) :
+    (toCNF'.run 0 x).1.eval (Sum.elim f (x.traceEval f)) = true := by
+  match x with
+  | .literal a => simp [toCNF'.run, traceEval, traceEval.run]
+  | .const b => simp [toCNF'.run, traceEval, traceEval.run]
+  | .not x =>
+    have := x.size_pos
+    have := toCNF'_run_fst_eval_elim_traceEval x f
+    revert this
+    simp only [toCNF'.run, toCNF'_run_snd, Nat.zero_add, CNF.eval_append, CNF.ne_eval, Sum.elim_inr,
+      traceEval, traceEval.run, Nat.succ.injEq, Bool.and_eq_true, beq_iff_eq]
+    rw [traceEval_run_snd_fst_of_le, traceEval_run_snd_fst, traceEval_run_fst, traceEval_run_fst]
+    have : CNF.eval (Sum.elim f (traceEval (not x) f)) (toCNF'.run 0 x).fst = CNF.eval (Sum.elim f (traceEval x f)) (toCNF'.run 0 x).fst := sorry
+    rw [this]
+    simp only [cond_false, cond_true, true_and, imp_self]
+    all_goals omega
+  | .gate g x y => sorry
+
+theorem toCNF'_eval_elim_traceEval (x : BoolExpr α) (f : α → Bool) :
+    (toCNF' x).eval (Sum.elim f (x.traceEval f)) = x.eval f := by
+  match x with
+  | .literal a => simp [toCNF', toCNF'.run, traceEval, traceEval.run]
+  | .const b => simp [toCNF', toCNF'.run, traceEval, traceEval.run]
+  | .not x =>
+    dsimp [toCNF']
+    have := toCNF'_run_fst_eval_elim_traceEval x f
+    revert this
+    simp [toCNF'.run]
+    have : CNF.eval (Sum.elim f (traceEval (not x) f)) (toCNF'.run 0 x).fst = CNF.eval (Sum.elim f (traceEval x f)) (toCNF'.run 0 x).fst := sorry
+    rw [this]
+    generalize CNF.eval (Sum.elim f (traceEval x f)) (toCNF'.run 0 x).fst = x1
+    cases x1 <;> simp
+    sorry
+  | .gate g x y => sorry
 
 theorem toCNF'_unsat {x : BoolExpr α} : (toCNF' x).unsat ↔ x.unsat := by
   constructor
@@ -122,7 +313,11 @@ theorem toCNF'_unsat {x : BoolExpr α} : (toCNF' x).unsat ↔ x.unsat := by
     rwa [toCNF'_eval_elim_traceEval] at h
   · intro h f
     specialize h (fun a => f (.inl a))
-    rwa [toCNF'_eval]
+    revert h
+    have := toCNF'_eval x f
+    revert this
+    cases CNF.eval f (toCNF' x) <;> cases eval (fun a => f (Sum.inl a)) x <;> simp
+
 
 def toCNF (x : BoolExpr Nat) : CNF Nat :=
   (toCNF' x.attach).relabel fun | .inl a => a | .inr j => x.vars + j
